Nel.v
@@ -1,0 +1,34 @@
+Add Rec LoadPath "/home/zeimer/Code/Coq".
+
+Require Import Cat.
+
+Inductive nel (A : Type) : Type :=
+    | singl : A -> nel A
+    | cons_nel : A -> nel A -> nel A.
+
+Arguments singl [A] _.
+Arguments cons_nel [A] _ _.
+
+Notation "h ::: t" := (cons_nel h t) (right associativity, at level 30).
+
+Fixpoint nel_app {A : Type} (l1 l2 : nel A) : nel A :=
+match l1 with
+    | singl a => cons_nel a l2
+    | a ::: l1' => cons_nel a (nel_app l1' l2)
+end.
+
+Notation "l1 +++ l2" := (nel_app l1 l2) (at level 40).
+
+Theorem app_nel_assoc : forall (A : Type) (x y z : nel A),
+    x +++ (y +++ z) = (x +++ y) +++ z.
+Proof.
+  induction x as [h | h t]; simpl; intros.
+    trivial.
+    rewrite IHt. trivial.
+Qed.
+
+Fixpoint nel_map {A B : Type} (f : A -> B) (l : nel A) : nel B :=
+match l with
+    | singl x => singl (f x)
+    | h ::: t => f h ::: nel_map f t
+end.
